common/Allocator.v
@@ -1,0 +1,780 @@
+Require Import Zwf.
+Require Import Axioms.
+Require Import Coqlib.
+Require Intv.
+Require Import Maps.
+Require Archi.
+Require Import AST.
+Require Import Integers.
+Require Import Floats.
+Require Import Values.
+Require Import Tags.
+Require Export Memdata.
+Require Import Memory.
+
+Require Import List. Import ListNotations.
+
+(* To avoid useless definitions of inductors in extracted code. *)
+Local Unset Elimination Schemes.
+Local Unset Case Analysis Schemes.
+
+Local Notation "a # b" := (PMap.get b a) (at level 1).
+
+Notation "'do' X <- A ; B" := (match A with Some X => B | None => None end)
+  (at level 200, X name, A at level 100, B at level 200)
+  : option_monad_scope.
+
+Notation "'do' X , Y <- A ; B" := (match A with Some (X, Y) => B | None => None end)
+  (at level 200, X name, Y name, A at level 100, B at level 200)
+  : option_monad_scope.
+
+Notation "'do' X , Y , Z <- A ; B" := (match A with Some (X, Y, Z) => B | None => None end)
+  (at level 200, X name, Y name, Z name, A at level 100, B at level 200)
+  : option_monad_scope.
+
+Notation "'do' X , Y , Z , W <- A ; B" := (match A with Some (X, Y, Z, W) => B | None => None end)
+  (at level 200, X name, Y name, Z name, W name, A at level 100, B at level 200)
+  : option_monad_scope.
+
+Notation "'check' A ; B" := (if A then B else None)
+  (at level 200, A at level 100, B at level 200)
+  : option_monad_scope.
+
+Open Scope option_monad_scope.
+
+Module Type Allocator (P : Policy).
+  Module Mem := Mem P.
+  Import Mem.
+  Export Memdata.
+  Import P.
+  
+  Parameter t : Type.  
+  Parameter init : t.
+  Definition mem : Type := (Mem.mem * t).
+  Definition empty := (Mem.empty, init).
+  
+  Parameter stkalloc : mem -> Z -> MemoryResult (mem * Z * Z).
+  Parameter stkfree : mem -> Z -> MemoryResult mem.
+  Parameter heapalloc : mem -> Z -> tag -> tag -> tag -> MemoryResult (mem * Z * Z).
+  Parameter heapfree : mem -> Z -> (tag -> PolicyResult (tag * tag * tag * tag)) ->
+                       MemoryResult (PolicyResult (tag*mem)).
+  Parameter globalalloc : mem -> list (ident*Z) -> (mem * PTree.t (Z * Z)).
+  
+  Definition load (chunk:memory_chunk) (m:mem) (addr:Z) := Mem.load chunk (fst m) addr.
+  Definition load_ltags (chunk:memory_chunk) (m:mem) (addr:Z) := Mem.load_ltags chunk (fst m) addr.
+  Definition load_all (chunk:memory_chunk) (m:mem) (addr:Z) := Mem.load_all chunk (fst m) addr.
+  Definition loadbytes (m:mem) (ofs n:Z) := Mem.loadbytes (fst m) ofs n.
+  
+  Definition store (chunk:memory_chunk) (m:mem) (addr:Z) (v:Mem.TLib.atom) (lts:list tag) :=
+    let (m,st) := m in
+    match Mem.store chunk m addr v lts with
+    | MemorySuccess m' => MemorySuccess (m',st)
+    | MemoryFail msg => MemoryFail msg
+    end.
+
+  Definition storebytes (m:mem) (ofs:Z) (bytes:list memval) (lts:list tag) :=
+    let (m,st) := m in
+    match Mem.storebytes m ofs bytes lts with
+    | MemorySuccess m' => MemorySuccess (m',st)
+    | MemoryFail msg => MemoryFail msg
+    end.
+  
+End Allocator.
+
+Module ConcreteAllocator (P : Policy) : Allocator P.
+  Module Mem := Mem P.
+  Import Mem.
+  Import P.
+
+  Definition t : Type := Z.
+  Definition init : t := 3000.
+  Definition mem : Type := (Mem.mem * t).
+  Definition empty := (Mem.empty, init).
+  
+  Definition stkalloc (m: mem) (size: Z) : MemoryResult (mem*Z*Z) :=
+    let '(m,sp) := m in
+    MemorySuccess ((m,sp-size),sp-size,sp).
+
+  Definition stkfree (m: mem) (size: Z) : MemoryResult mem :=
+    let '(m,sp) := m in
+    MemorySuccess (m,sp+size).
+
+  Definition check_record (m: Mem.mem) (base: Z) : option (bool * Z * tag) :=
+    match load Mint64 m base with
+    | MemorySuccess (Vlong i, vt) =>
+        let live := (0 <=? (Int64.signed i))%Z in
+        let sz := (Z.abs (Int64.signed i)) in
+        Some (live, sz, vt)
+    | _ => None
+    end.
+
+  Definition update_record (m: Mem.mem) (base: Z) (live: bool) (sz: Z) (vt: tag) (lt: tag)
+    : option Mem.mem :=
+    let rec :=
+      if live
+      then Vlong (Int64.repr sz)
+      else Vlong (Int64.neg (Int64.repr sz))
+    in
+    match store Mint64 m base (rec, vt) [lt;lt;lt;lt;lt;lt;lt;lt] with
+    | MemorySuccess m'' => Some m''
+    | MemoryFail _ => None
+    end.
+
+  Definition record_size := size_chunk Mint64.
+    
+  Fixpoint find_free (c : nat) (m : Mem.mem) (base : Z) (sz : Z) (vt lt : tag) : option (Mem.mem*Z) :=
+    match c with
+    | O => None
+    | S c' =>
+        (* Load a long from base.
+           Sign indictates: is this a live block? (Negative no, positive/zero yes)
+           Magnitude indicates size *)
+        match check_record m base with
+        | Some (true, bs, vt') =>
+            let next := base + bs in
+            find_free c' m next sz vt lt
+        | Some (false, bs, vt') =>
+            let remain := bs - sz in
+            if (remain <? 0)%Z then
+              let next := base + bs in find_free c' m next sz vt lt
+            else
+              if (record_size <? remain)%Z then
+                let next := base + bs in
+                let next_sz := remain - record_size in
+                do m' <- update_record m base false sz vt lt;
+                do m'' <- update_record m' next true next_sz def_tag def_tag;
+                Some (m'',base)
+              else
+                do m' <- update_record m base true bs vt lt;
+                Some (m',base)
+        | None => None
+        end
+    end.
+  
+  Definition heapalloc (m: mem) (size: Z) (vt_head vt_body lt: tag) : MemoryResult (mem * Z * Z) :=
+    let '(m,sp) := m in
+    match find_free 100 m 1000 size vt_head lt with
+    | Some (m', base) =>
+        match storebytes m' (base + record_size)
+                         (repeat (Byte Byte.zero vt_body) (Z.to_nat size))
+                         (repeat lt (Z.to_nat size)) with
+        | MemorySuccess m'' =>
+            MemorySuccess ((m'',sp), base + record_size, base + record_size + size)
+        | MemoryFail msg => MemoryFail msg
+        end
+    | None => MemoryFail "OOM"
+    end.
+
+
+(*        Definition do_ef_malloc_unsafe
+               (w: world) (vargs: list atom) (PCT: tag) (m: mem)
+      : option (world * trace * (MemoryResult (PolicyResult (atom * tag * mem)))) :=
+      match vargs with
+      | [(v,st)] =>
+          match MallocT PCT def_tag st with
+          | PolicySuccess (PCT',pt',vt1,vt2,lt) =>
+              do sz <- option_map Ptrofs.unsigned (do_alloc_size v);
+              do m', base <- find_free 100 m 1000 sz vt2 lt;
+              match storebytes m' (base + record_size)
+                               (repeat (Byte Byte.zero vt1) (Z.to_nat sz))
+                               (repeat lt (Z.to_nat sz)) with
+              | MemorySuccess m'' =>
+                  Some (w, E0, (MemorySuccess (PolicySuccess((Vlong (Int64.repr (base + record_size)), def_tag), PCT', m''))))
+              | MemoryFail msg => Some (w, E0, (MemoryFail msg))
+              end
+          | PolicyFail msg params =>
+              Some (w, E0, (MemorySuccess (PolicyFail msg params)))
+          end
+      | _ => None
+      end. *)
+
+  Definition heapfree (m: mem) (addr: Z) (rule : tag -> PolicyResult (tag*tag*tag*tag))
+    : MemoryResult (PolicyResult (tag * mem)) :=
+    let (m, sp) := m in
+    match check_record m (addr-record_size) with
+    | Some (live, sz, vt) =>
+        match rule vt with
+        | PolicySuccess (PCT', vt1, vt2, lt) =>
+            match update_record m (addr-record_size) false sz vt2 lt with
+            | Some m' =>
+                MemorySuccess (PolicySuccess (PCT', (m', sp)))
+            | None => MemoryFail "Free failing"
+            end
+        | PolicyFail msg params =>
+            MemorySuccess (PolicyFail msg params)
+        end
+    | None => MemoryFail "Free failing"
+    end.
+  
+  Fixpoint globals (m : Mem.mem) (gs : list (ident*Z)) (next : Z) : (Mem.mem * PTree.t (Z*Z)) :=
+    match gs with
+    | [] => (m, PTree.empty (Z*Z))
+    | (id,sz)::gs' =>
+        let (m',tree) := globals m gs' (next+sz) in
+        (set_perm_range m next (next+sz-1) Live, PTree.set id (next,next+sz-1) tree)
+    end.
+              
+  Definition globalalloc (m : mem) (gs : list (ident*Z)) : (mem * PTree.t (Z*Z)) :=
+    let (m, sp) := m in
+    let (m', tree) := globals m gs 4 in
+    ((m',sp), tree).
+  
+  Definition load (chunk:memory_chunk) (m:mem) (addr:Z) := Mem.load chunk (fst m) addr.
+  Definition load_ltags (chunk:memory_chunk) (m:mem) (addr:Z) := Mem.load_ltags chunk (fst m) addr.
+  Definition load_all (chunk:memory_chunk) (m:mem) (addr:Z) := Mem.load_all chunk (fst m) addr.
+  Definition loadbytes (m:mem) (ofs n:Z) := Mem.loadbytes (fst m) ofs n.
+  
+  Definition store (chunk:memory_chunk) (m:mem) (addr:Z) (v:Mem.TLib.atom) (lts:list tag) :=
+    let (m,sp) := m in
+    match Mem.store chunk m addr v lts with
+    | MemorySuccess m' => MemorySuccess (m',sp)
+    | MemoryFail msg => MemoryFail msg
+    end.
+
+  Definition storebytes (m:mem) (ofs:Z) (bytes:list memval) (lts:list tag) :=
+    let (m,st) := m in
+    match Mem.storebytes m ofs bytes lts with
+    | MemorySuccess m' => MemorySuccess (m',st)
+    | MemoryFail msg => MemoryFail msg
+    end.
+  
+End ConcreteAllocator.
+  
+Module FLAllocator (P : Policy) : Allocator P.
+  Module Mem := Mem P.
+  Import Mem.
+  Import P.  
+  
+  Definition freelist : Type := list (Z*Z).
+
+  Record heap_state : Type := mkheap {
+    regions : ZMap.t (option (Z*tag));
+    fl : freelist;
+  }.
+
+  Definition empty_heap : heap_state :=
+    mkheap (ZMap.init None) [(1000,2000)].
+  
+  Definition t : Type := (Z*heap_state).   
+  Definition init : t := (3000,empty_heap).  
+  Definition mem : Type := (Mem.mem * t).
+  Definition empty := (Mem.empty, init).
+  
+  (** Allocation of a fresh block with the given bounds.  Return an updated
+      memory state and the address of the fresh block, which initially contains
+      undefined cells.  Note that allocation never fails: we model an
+      infinite memory. *)
+  Definition stkalloc (m: mem) (size: Z) : MemoryResult (mem*Z*Z) :=
+    let '(m,(sp,heap)) := m in
+    MemorySuccess ((m,(sp-size,heap)),sp-size,sp).
+
+  Definition stkfree (m: mem) (size: Z) : MemoryResult mem :=
+    let '(m,(sp,heap)) := m in
+    MemorySuccess (m,(sp+size,heap)).
+  
+  Fixpoint fl_alloc (fl : freelist) (size : Z) : option (Z*Z*freelist) :=
+    match fl with
+    | [] => None
+    | (base, bound) :: fl' =>
+        if bound - base =? size
+        then Some (base,bound,fl')
+        else if size <? bound - base
+             then Some (base,base+size,(base+size+1,bound)::fl')
+             else match fl_alloc fl' size with
+                  | Some (base',bound',fl'') => Some (base', bound', (base, bound) :: fl'')
+                  | None => None
+                  end
+    end.
+  
+  Definition heapalloc (m : mem) (size : Z) (vt_head vt_body lt : tag) : MemoryResult (mem*Z*Z) :=
+    let '(m, (sp,heap)) := m in
+    match fl_alloc heap.(fl) size with
+    | Some (base, bound, fl') =>
+        let regions' := ZMap.set base (Some (bound,vt_head)) heap.(regions) in
+        MemorySuccess ((m, (sp, mkheap regions' fl')), base, bound)
+    | None => MemoryFail "Out of memory"
+    end.
+
+  Definition heapfree (m : mem) (base : Z) (rule : tag -> PolicyResult (tag*tag*tag*tag))
+    : MemoryResult (PolicyResult (tag*mem)) :=
+    let '(m, (sp,heap)) := m in
+    match ZMap.get base heap.(regions) with
+    | Some (bound,vt) =>
+        match rule vt with
+        | PolicySuccess (pct',vt_head,vt_body,lt) =>
+            let heap' := (mkheap (ZMap.set base None heap.(regions))
+                                 ((base,bound)::heap.(fl))) in
+            MemorySuccess (PolicySuccess (pct', (m, (sp,heap'))))
+        | PolicyFail msg params =>
+            MemorySuccess (PolicyFail msg params)
+        end
+    | None => MemoryFail "Bad free"
+    end.
+
+  Fixpoint globals (m : Mem.mem) (gs : list (ident*Z)) (next : Z) : (Mem.mem * PTree.t (Z*Z)) :=
+    match gs with
+    | [] => (m, PTree.empty (Z*Z))
+    | (id,sz)::gs' =>
+        let (m',tree) := globals m gs' (next+sz) in
+        (set_perm_range m next (next+sz-1) Live, PTree.set id (next,next+sz-1) tree)
+    end.
+              
+  Definition globalalloc (m : mem) (gs : list (ident*Z)) : (mem * PTree.t (Z*Z)) :=
+    let (m, sp) := m in
+    let (m', tree) := globals m gs 4 in
+    ((m',sp), tree).
+  
+  Definition load (chunk:memory_chunk) (m:mem) (addr:Z) := Mem.load chunk (fst m) addr.
+  Definition load_ltags (chunk:memory_chunk) (m:mem) (addr:Z) := Mem.load_ltags chunk (fst m) addr.
+  Definition load_all (chunk:memory_chunk) (m:mem) (addr:Z) := Mem.load_all chunk (fst m) addr.
+  Definition loadbytes (m:mem) (ofs n:Z) := Mem.loadbytes (fst m) ofs n.
+
+  Definition store (chunk:memory_chunk) (m:mem) (addr:Z) (v:Mem.TLib.atom) (lts:list tag) :=
+    let (m,sp) := m in
+    match Mem.store chunk m addr v lts with
+    | MemorySuccess m' => MemorySuccess (m',sp)
+    | MemoryFail msg => MemoryFail msg
+    end.
+
+  Definition storebytes (m:mem) (ofs:Z) (bytes:list memval) (lts:list tag) :=
+    let (m,st) := m in
+    match Mem.storebytes m ofs bytes lts with
+    | MemorySuccess m' => MemorySuccess (m',st)
+    | MemoryFail msg => MemoryFail msg
+    end.
+  
+End FLAllocator.
+  
+(*Section ALLOC.
+
+Variable m1: mem.
+Variables lo1 lo2 hi1 hi2: Z.
+Variable m2: mem.
+Hypothesis ALLOC: alloc m1 lo1 hi1 = MemorySuccess (m2, lo2, hi2).
+
+Ltac alloc_inv :=
+  let p := fresh "p" in
+  unfold alloc in ALLOC;
+  destruct (al.(stkalloc) m1.(al_state) (hi1 - lo1)) as [p |];
+  repeat destruct p;
+  inv ALLOC.
+
+Theorem valid_block_alloc:
+  forall ofs, valid_addr m1 ofs -> valid_addr m2 ofs.
+Proof.
+  unfold valid_addr; intros. destruct H as [lo [hi H]]. exists lo. exists hi.
+  unfold alloc in *.
+  destruct (stkalloc al (al_state m1) (hi1-lo1)) as [res |]; [|inv ALLOC].
+  destruct res as [[al_state' lo'] hi']. inv ALLOC.
+  simpl. destruct H. split;[right|]; auto.
+Qed.
+
+Theorem valid_new_block:
+  forall ofs, lo2 <= ofs -> ofs < hi2 -> valid_addr m2 ofs.
+Admitted.
+
+Local Hint Resolve valid_block_alloc valid_new_block : mem.
+
+Theorem valid_block_alloc_inv:
+  forall addr, valid_addr m2 addr -> (lo2 <= addr /\ addr < hi2) \/ valid_addr m1 addr.
+Admitted.
+(*Proof.
+  unfold valid_addr; intros.
+  destruct (lo2 <=? addr); [right | destruct (addr <? hi2); [left | right]].
+  - destruct H as [lo [hi H]]. exists lo. exists hi.
+    unfold alloc in *.
+    destruct (stkalloc al (al_state m1) (hi1-lo1)) as [res|]; [|inv ALLOC].
+    destruct res as [[al_state' lo'] hi']. inv ALLOC.
+    simpl in *. auto.
+Qed.*)
+
+(*Theorem perm_alloc_1:
+  forall ofs k p, perm m1 ofs k p -> perm m2 ofs k p.
+Proof.
+  unfold perm; intros. alloc_inv. simpl.
+  rewrite PMap.gsspec. destruct (peq b); auto.
+  destruct (zle lo2 ofs && zlt ofs hi); eauto.
+  rewrite nextblock_noaccess in H. contradiction. apply Plt_strict.
+Qed.
+
+Theorem perm_alloc_2:
+  forall ofs k, lo2 <= ofs < hi2 -> perm m2 ofs k Freeable.
+Proof.
+  unfold perm; intros. injection ALLOC; intros. rewrite <- H1; simpl.
+  subst b. rewrite PMap.gss. unfold proj_sumbool. rewrite zle_true.
+  rewrite zlt_true. simpl. auto with mem. lia. lia.
+Qed.
+
+Theorem perm_alloc_inv:
+  forall ofs k p,
+  perm m2 ofs k p ->
+  if eq_block then lo2 <= ofs < hi2 else perm m1 ofs k p.
+Proof.
+  intros until p; unfold perm. inv ALLOC. simpl.
+  rewrite PMap.gsspec. unfold eq_block. destruct (peq (nextblock m1)); intros.
+  destruct (zle lo2 ofs); try contradiction. destruct (zlt ofs hi); try contradiction.
+  split; auto.
+  auto.
+Qed.
+
+Theorem perm_alloc_3:
+  forall ofs k p, perm m2 ofs k p -> lo2 <= ofs < hi.
+Proof.
+  intros. exploit perm_alloc_inv; eauto. rewrite dec_eq_true; auto.
+Qed.
+
+Theorem perm_alloc_4:
+  forall ofs k p, perm m2 ofs k p -> <> -> perm m1 ofs k p.
+Proof.
+  intros. exploit perm_alloc_inv; eauto. rewrite dec_eq_false; auto.
+Qed.
+
+Local Hint Resolve perm_alloc_1 perm_alloc_2 perm_alloc_3 perm_alloc_4: mem.
+*)
+
+(*Theorem valid_access_alloc_other:
+  forall chunk ofs p,
+  valid_access m1 chunk ofs p ->
+  valid_access m2 chunk ofs p.
+Proof.
+  intros. inv H. constructor; auto with mem.
+  red; auto with mem.
+Qed.
+
+Theorem valid_access_alloc_same:
+  forall chunk ofs,
+  lo2 <= ofs -> ofs + size_chunk chunk <= hi2 -> (align_chunk chunk | ofs) ->
+  valid_access m2 chunk ofs Freeable.
+Proof.
+  intros. constructor; auto with mem.
+  red; intros. apply perm_alloc_2. lia.
+Qed.
+
+Local Hint Resolve valid_access_alloc_other valid_access_alloc_same: mem.
+
+Theorem valid_access_alloc_inv:
+  forall chunk ofs p,
+  valid_access m2 chunk ofs p ->
+  if eq_block b
+  then lo2 <= ofs /\ ofs + size_chunk chunk <= hi2 /\ (align_chunk chunk | ofs)
+  else valid_access m1 chunk ofs p.
+Proof.
+  intros. inv H.
+  generalize (size_chunk_pos chunk); intro.
+  destruct (eq_block b). subst b'.
+  assert (perm m2 ofs Cur p). apply H0. lia.
+  assert (perm m2 (ofs + size_chunk chunk - 1) Cur p). apply H0. lia.
+  exploit perm_alloc_inv. eexact H2. rewrite dec_eq_true. intro.
+  exploit perm_alloc_inv. eexact H3. rewrite dec_eq_true. intro.
+  intuition lia.
+  split; auto. red; intros.
+  exploit perm_alloc_inv. apply H0. eauto. rewrite dec_eq_false; auto.
+Qed.
+ 
+
+Theorem load_alloc_unchanged:
+  forall chunk ofs,
+  valid_block m1 ->
+  load chunk m2 ofs = load chunk m1 ofs.
+Proof.
+  intros. unfold load.
+  destruct (valid_access_dec m2 chunk ofs Readable).
+  exploit valid_access_alloc_inv; eauto. destruct (eq_block b); intros.
+  subst b'. elimtype False. eauto with mem.
+  rewrite pred_dec_true; auto.
+  injection ALLOC; intros. rewrite <- H2; simpl.
+  rewrite PMap.gso. auto. rewrite H1. apply not_eq_sym; eauto with mem.
+  rewrite pred_dec_false. auto.
+  eauto with mem.
+Qed.
+
+Theorem load_alloc_other:
+  forall chunk ofs v,
+  load chunk m1 ofs = Some v ->
+  load chunk m2 ofs = Some v.
+Proof.
+  intros. rewrite <- H. apply load_alloc_unchanged. eauto with mem.
+Qed.
+
+Theorem load_alloc_same:
+  forall chunk ofs v,
+  load chunk m2 ofs = Some v ->
+  v = Vundef.
+Proof.
+  intros. exploit load_result; eauto. intro. rewrite H0.
+  injection ALLOC; intros. rewrite <- H2; simpl. rewrite <- H1.
+  rewrite PMap.gss. destruct (size_chunk_nat_pos chunk) as [n E]. rewrite E. simpl.
+  rewrite ZMap.gi. apply decode_val_undef.
+Qed.
+
+Theorem load_alloc_same':
+  forall chunk ofs,
+  lo2 <= ofs -> ofs + size_chunk chunk <= hi2 -> (align_chunk chunk | ofs) ->
+  load chunk m2 ofs = Some Vundef.
+Proof.
+  intros. assert (exists v, load chunk m2 ofs = Some v).
+    apply valid_access_load. constructor; auto.
+    red; intros. eapply perm_implies. apply perm_alloc_2. lia. auto with mem.
+  destruct H2 as [v LOAD]. rewrite LOAD. decEq.
+  eapply load_alloc_same; eauto.
+Qed.
+
+Theorem loadbytes_alloc_unchanged:
+  forall ofs n,
+  valid_block m1 ->
+  loadbytes m2 ofs n = loadbytes m1 ofs n.
+Proof.
+  intros. unfold loadbytes.
+  destruct (range_perm_dec m1 ofs (ofs + n) Cur Readable).
+  rewrite pred_dec_true.
+  injection ALLOC; intros A B. rewrite <- B; simpl.
+  rewrite PMap.gso. auto. rewrite A. eauto with mem.
+  red; intros. eapply perm_alloc_1; eauto.
+  rewrite pred_dec_false; auto.
+  red; intros; elim n0. red; intros. eapply perm_alloc_4; eauto. eauto with mem.
+Qed.
+
+Theorem loadbytes_alloc_same:
+  forall n ofs bytes byte,
+  loadbytes m2 ofs n = Some bytes ->
+  In byte bytes -> byte = Undef.
+Proof.
+  unfold loadbytes; intros. destruct (range_perm_dec m2 ofs (ofs + n) Cur Readable); inv H.
+  revert H0.
+  injection ALLOC; intros A B. rewrite <- A; rewrite <- B; simpl. rewrite PMap.gss.
+  generalize (Z.to_nat n) ofs. induction n0; simpl; intros.
+  contradiction.
+  rewrite ZMap.gi in H0. destruct H0; eauto.
+Qed.
+*)
+End ALLOC.
+
+Local Hint Resolve valid_block_alloc : mem.
+(*Local Hint Resolve valid_access_alloc_other valid_access_alloc_same: mem.*)
+
+(** ** Properties related to [free]. *)
+
+Theorem range_perm_free:
+  forall m1 lo hi,
+  range_perm m1 lo hi Live ->
+  { m2: mem | free m1 lo hi = MemorySuccess m2 }.
+Proof.
+  intros; unfold free. rewrite pred_dec_true; auto. econstructor; eauto.
+Defined.
+
+Section FREE.
+
+Variable m1: mem.
+Variables lo hi: Z.
+Variable m2: mem.
+Hypothesis FREE: free m1 lo hi = MemorySuccess m2.
+
+Theorem free_range_perm:
+  range_perm m1 lo hi Live.
+Proof.
+  unfold free in FREE. destruct (range_perm_dec m1 lo hi Live); auto.
+  congruence.
+Qed.
+
+Lemma free_result:
+  m2 = unchecked_free m1 lo hi.
+Proof.
+  unfold free in FREE. destruct (range_perm_dec m1 lo hi Live).
+  congruence. congruence.
+Qed.
+
+Theorem valid_block_free_1:
+  forall ofs,
+    (lo > ofs \/ hi <= ofs) ->
+    valid_addr m1 ofs ->
+    valid_addr m2 ofs.
+Admitted.
+(*Proof.
+  intros. rewrite free_result.
+  unfold unchecked_free.
+  assumption.
+Qed.*)
+
+Theorem valid_block_free_2:
+  forall ofs, valid_addr m2 ofs -> valid_addr m1 ofs.
+Admitted.
+(*Proof.
+  intros. rewrite free_result in H. assumption.
+Qed.*)
+
+Local Hint Resolve valid_block_free_1 valid_block_free_2: mem.
+
+(*Theorem perm_free_1:
+  forall ofs k p,
+  <> \/ ofs < lo \/ hi <= ofs ->
+  perm m1 ofs k p ->
+  perm m2 ofs k p.
+Proof.
+  intros. rewrite free_result. unfold perm, unchecked_free; simpl.
+  rewrite PMap.gsspec. destruct (peq bf). subst b.
+  destruct (zle lo ofs); simpl.
+  destruct (zlt ofs hi); simpl.
+  elimtype False; intuition.
+  auto. auto.
+  auto.
+Qed.
+
+Theorem perm_free_2:
+  forall ofs k p, lo <= ofs < hi -> ~ perm m2 ofs k p.
+Proof.
+  intros. rewrite free_result. unfold perm, unchecked_free; simpl.
+  rewrite PMap.gss. unfold proj_sumbool. rewrite zle_true. rewrite zlt_true.
+  simpl. tauto. lia. lia.
+Qed.
+
+Theorem perm_free_3:
+  forall ofs k p,
+  perm m2 ofs k p -> perm m1 ofs k p.
+Proof.
+  intros until p. rewrite free_result. unfold perm, unchecked_free; simpl.
+  rewrite PMap.gsspec. destruct (peq bf). subst b.
+  destruct (zle lo ofs); simpl.
+  destruct (zlt ofs hi); simpl. tauto.
+  auto. auto. auto.
+Qed.
+
+Theorem perm_free_inv:
+  forall ofs k p,
+  perm m1 ofs k p ->
+  (= /\ lo <= ofs < hi) \/ perm m2 ofs k p.
+Proof.
+  intros. rewrite free_result. unfold perm, unchecked_free; simpl.
+  rewrite PMap.gsspec. destruct (peq bf); auto. subst b.
+  destruct (zle lo ofs); simpl; auto.
+  destruct (zlt ofs hi); simpl; auto.
+Qed.
+
+Theorem valid_access_free_1:
+  forall chunk ofs p,
+  valid_access m1 chunk ofs p ->
+  <> \/ lo >= hi \/ ofs + size_chunk chunk <= lo \/ hi <= ofs ->
+  valid_access m2 chunk ofs p.
+Proof.
+  intros. inv H. constructor; auto with mem.
+  red; intros. eapply perm_free_1; eauto.
+  destruct (zlt lo hi). intuition. right. lia.
+Qed.
+
+Theorem valid_access_free_2:
+  forall chunk ofs p,
+  lo < hi -> ofs + size_chunk chunk > lo -> ofs < hi ->
+  ~(valid_access m2 chunk ofs p).
+Proof.
+  intros; red; intros. inv H2.
+  generalize (size_chunk_pos chunk); intros.
+  destruct (zlt ofs lo).
+  elim (perm_free_2 lo Cur p).
+  lia. apply H3. lia.
+  elim (perm_free_2 ofs Cur p).
+  lia. apply H3. lia.
+Qed.
+
+Theorem valid_access_free_inv_1:
+  forall chunk ofs p,
+  valid_access m2 chunk ofs p ->
+  valid_access m1 chunk ofs p.
+Proof.
+  intros. destruct H. split; auto.
+  red; intros. generalize (H ofs0 H1).
+  rewrite free_result. unfold perm, unchecked_free; simpl.
+  rewrite PMap.gsspec. destruct (peq bf). subst b.
+  destruct (zle lo ofs0); simpl.
+  destruct (zlt ofs0 hi); simpl.
+  tauto. auto. auto. auto.
+Qed.
+
+Theorem valid_access_free_inv_2:
+  forall chunk ofs p,
+  valid_access m2 chunk ofs p ->
+  lo >= hi \/ ofs + size_chunk chunk <= lo \/ hi <= ofs.
+Proof.
+  intros.
+  destruct (zlt lo hi); auto.
+  destruct (zle (ofs + size_chunk chunk) lo); auto.
+  destruct (zle hi ofs); auto.
+  elim (valid_access_free_2 chunk ofs p); auto. lia.
+Qed.
+
+Theorem load_free:
+  forall chunk ofs,
+  <> \/ lo >= hi \/ ofs + size_chunk chunk <= lo \/ hi <= ofs ->
+  load chunk m2 ofs = load chunk m1 ofs.
+Proof.
+  intros. unfold load.
+  destruct (valid_access_dec m2 chunk ofs Readable).
+  rewrite pred_dec_true.
+  rewrite free_result; auto.
+  eapply valid_access_free_inv_1; eauto.
+  rewrite pred_dec_false; auto.
+  red; intro; elim n. eapply valid_access_free_1; eauto.
+Qed.
+
+Theorem load_free_2:
+  forall chunk ofs v,
+  load chunk m2 ofs = Some v -> load chunk m1 ofs = Some v.
+Proof.
+  intros. unfold load. rewrite pred_dec_true.
+  rewrite (load_result _ _ _ _ _ H). rewrite free_result; auto.
+  apply valid_access_free_inv_1. eauto with mem.
+Qed.
+
+Theorem loadbytes_free:
+  forall ofs n,
+  <> \/ lo >= hi \/ ofs + n <= lo \/ hi <= ofs ->
+  loadbytes m2 ofs n = loadbytes m1 ofs n.
+Proof.
+  intros. unfold loadbytes.
+  destruct (range_perm_dec m2 ofs (ofs + n) Cur Readable).
+  rewrite pred_dec_true.
+  rewrite free_result; auto.
+  red; intros. eapply perm_free_3; eauto.
+  rewrite pred_dec_false; auto.
+  red; intros. elim n0; red; intros.
+  eapply perm_free_1; eauto. destruct H; auto. right; lia.
+Qed.
+
+Theorem loadbytes_free_2:
+  forall ofs n bytes,
+  loadbytes m2 ofs n = Some bytes -> loadbytes m1 ofs n = Some bytes.
+Proof.
+  intros. unfold loadbytes in *.
+  destruct (range_perm_dec m2 ofs (ofs + n) Cur Readable); inv H.
+  rewrite pred_dec_true. rewrite free_result; auto.
+  red; intros. apply perm_free_3; auto.
+Qed.
+*)
+End FREE.
+
+Global Opaque Mem.alloc Mem.free.
+
+Global Hint Resolve
+  (*Mem.alloc_result*)
+  Mem.valid_block_alloc
+  Mem.valid_new_block
+  (*Mem.perm_alloc_1
+  Mem.perm_alloc_2
+  Mem.perm_alloc_3
+  Mem.perm_alloc_4
+  Mem.perm_alloc_inv*)
+  (*Mem.valid_access_alloc_other
+  Mem.valid_access_alloc_same
+  Mem.valid_access_alloc_inv*)
+  Mem.range_perm_free
+  Mem.free_range_perm
+  Mem.valid_block_free_1
+  Mem.valid_block_free_2
+  (*Mem.perm_free_1
+  Mem.perm_free_2
+  Mem.perm_free_3
+  Mem.valid_access_free_1
+  Mem.valid_access_free_2
+  Mem.valid_access_free_inv_1
+  Mem.valid_access_free_inv_2
+  Mem.unchanged_on_refl*)
+  : al.
+*)
