common/Layout.v
@@ -1,0 +1,10 @@
+Require Import ZArith.
+
+Module Type Layout.
+  Parameter global_min : Z.
+  Parameter global_max : Z.
+  Parameter heap_min : Z.
+  Parameter heap_max : Z.
+  Parameter stack_min : Z.
+  Parameter stack_max : Z.
+End Layout.
